Finish the monster that is parse-tree minimization

src/Parsers/MinimalParse.v
@@ -323,9 +323,9 @@ Section cfg.
       eapply not_alt_all; eassumption.
     Defined.
 
-    Definition expand_alt_option {h h' str valid valid'}
-               (H : h < h') (H' : sub_productions_listT valid' valid)
-    : alt_option h valid str -> alt_option h' valid' str.
+    Definition expand_alt_option {h h' str str' valid valid'}
+               (H : h < h') (H' : sub_productions_listT valid' valid) (H'' : str = str')
+    : alt_option h valid str -> alt_option h' valid' str'.
     Proof.
       hnf in H'; unfold alt_option.
       repeat match goal with
@@ -334,6 +334,7 @@ Section cfg.
                | [ |- prod _ _ -> _ ] => intros []
                | [ |- and _ _ -> _ ] => intros []
                | _ => intro
+               | _ => progress subst
                | [ |- sigT _ ] => esplit
                | [ |- sig _ ] => esplit
                | [ |- prod _ _ ] => esplit
@@ -381,15 +382,19 @@ Section cfg.
     Defined.*)
 
     Section wf_parts.
-      Let of_parse_T h
-        := forall {str : String} (valid : productions_listT) {pats : productions CharType}
-                  (p : parse_of String G str pats)
-                  (p_small : height_of_parse p < h),
+      Let of_parse_T' h
+          {str : String} (valid : productions_listT) {pats : productions CharType}
+          (p : parse_of String G str pats)
+
+        := forall (p_small : height_of_parse p < h),
              Forall_parse_of P p
              -> ({ p' : minimal_parse_of valid str pats
                         & (height_of_parse (parse_of__of__minimal_parse_of p') <= height_of_parse p)
                           * Forall_parse_of P (parse_of__of__minimal_parse_of p') })%type
                 + alt_option (height_of_parse p) valid str.
+
+      Let of_parse_T h
+        := forall {str} valid {pats} p, @of_parse_T' h str valid pats p.
 
       Definition of_parse_T_resp {h h'} (H : h' < h) (parse : of_parse_T h)
       : of_parse_T h'
@@ -486,6 +491,7 @@ Section cfg.
                                                   => inr (expand_alt_option
                                                             (Lt.lt_n_S _ _ (fst (projT2 (snd other'))))
                                                             (reflexivity _)
+                                                            (reflexivity _)
                                                             p''')
                                               end
                                          | right H'
@@ -529,9 +535,6 @@ Section cfg.
         Let rec_T h
           := forall h', h' < h -> of_parse_T h' -> forall str valid pat p, @of_parse_production_T str valid pat p h'.
 
-        Context {str : String} (valid : productions_listT) {pat : production CharType}.
-
-
         Section helper.
           Context (h : nat)
                   (minimal_parse_of_production__of__parse_of_production_rec : rec_T h)
@@ -543,8 +546,10 @@ Section cfg.
             := @minimal_parse_of_production__of__parse_of_production_rec
                  h' H (of_parse_T_resp H (@minimal_parse_of__of__parse_of)).
 
-          Let minimal_parse_of_item__of__parse_of_item {str valid it}
+          Let minimal_parse_of_item__of__parse_of_item {str} valid {it}
             := @minimal_parse_of_item__of__parse_of_item' str valid it h minimal_parse_of__of__parse_of.
+
+          Context {str : String} (valid : productions_listT) {pat : production CharType}.
 
           Definition minimal_parse_of_production__of__parse_of_production'_helper
                      (p : parse_of_production String G str pat)
@@ -573,1049 +578,192 @@ Section cfg.
                           match stringlike_dec str0 (Empty _), stringlike_dec str1 (Empty _) with
                             | right pf0, right pf1
                               => inl (existT
-                                        _ (MinParseProductionConsDec valid pf0 pf1 _ (*mp0'*) _(*mp1'*))
-                                        _)
+                                        _ (MinParseProductionConsDec valid pf0 pf1 (projT1 mp0') (projT1 mp1'))
+                                        (NPeano.Nat.max_le_compat _ _ _ _ (Le.le_n_S _ _ (fst (projT2 mp0'))) (Le.le_n_S _ _ (fst (projT2 mp1'))),
+                                         (snd (projT2 mp0'), snd (projT2 mp1'))))
                             | left pf0, left pf1
                               => let eq_pf0 := (_ : str0 = str0 ++ str1) in
                                  let eq_pf1 := (_ : str1 = str0 ++ str1) in
                                  match mp0, mp1 with
                                    | inl mp0'', inl mp1''
                                      => inl (existT
-                                               _ (MinParseProductionConsEmpty01 pf0 pf1 _(*mp0''*) _(*mp1''*))
-                                               _)
+                                               _ (MinParseProductionConsEmpty01 pf0 pf1 (projT1 mp0'') (projT1 mp1''))
+                                               (NPeano.Nat.max_le_compat _ _ _ _ (Le.le_n_S _ _ (fst (projT2 mp0''))) (Le.le_n_S _ _ (fst (projT2 mp1''))),
+                                                (snd (projT2 mp0''), snd (projT2 mp1''))))
                                    | inr other, _
-                                     => inr (match eq_pf0 in (_ = str1) return (alt_option _ valid str1) with
-                                               | eq_refl => _(*other*)
-                                             end)
+                                     => inr (expand_alt_option
+                                               (Max.le_max_l _ _)
+                                               (reflexivity _)
+                                               eq_pf0
+                                               other)
                                    | _, inr other
-                                     => inr (match eq_pf1 in (_ = str1) return (alt_option _ valid str1) with
-                                               | eq_refl => _(*other*)
-                                             end)
+                                     => inr (expand_alt_option
+                                               (Max.le_max_r _ _)
+                                               (reflexivity _)
+                                               eq_pf1
+                                               other)
                                  end
                             | left pf0, right pf1
                               => let eq_pf := (_ : str1 = str0 ++ str1) in
                                  match mp1 with
                                    | inl mp1''
                                      => inl (existT
-                                               _ (MinParseProductionConsEmpty0 pf0 pf1 _(*mp0'*) _(*mp1''*))
-                                               _)
+                                               _ (MinParseProductionConsEmpty0 pf0 pf1 (projT1 mp0') (projT1 mp1''))
+                                               (NPeano.Nat.max_le_compat _ _ _ _ (Le.le_n_S _ _ (fst (projT2 mp0'))) (Le.le_n_S _ _ (fst (projT2 mp1''))),
+                                                (snd (projT2 mp0'), snd (projT2 mp1''))))
                                    | inr other
-                                     => inr (match eq_pf in (_ = str0) return (alt_option _ valid str0) with
-                                               | eq_refl => _(*other*)
-                                             end)
+                                     => inr (expand_alt_option
+                                               (Max.le_max_r _ _)
+                                               (reflexivity _)
+                                               eq_pf
+                                               other)
                                  end
                             | right pf0, left pf1
                               => let eq_pf := (_ : str0 = str0 ++ str1) in
-                                 _ (*match mp0 with
-                           | inl mp0''
-                             => inl (MinParseProductionConsEmpty1 pf0 pf1 mp0'' mp1')
-                           | inr other
-                             => inr (match eq_pf in (_ = str0) return (alt_option valid str0) with
-                                       | eq_refl => other
-                                     end)
-                         end*)
+                                 match mp0 with
+                                   | inl mp0''
+                                     => inl (existT
+                                               _ (MinParseProductionConsEmpty1 pf0 pf1 (projT1 mp0'') (projT1 mp1'))
+                                               (NPeano.Nat.max_le_compat _ _ _ _ (Le.le_n_S _ _ (fst (projT2 mp0''))) (Le.le_n_S _ _ (fst (projT2 mp1'))),
+                                                (snd (projT2 mp0''), snd (projT2 mp1'))))
+                                   | inr other
+                                     => inr (expand_alt_option
+                                               (Max.le_max_l _ _)
+                                               (reflexivity _)
+                                               eq_pf
+                                               other)
+                                 end
                           end
                 end
                   (@minimal_parse_of_production__of__parse_of_production)
                   (@minimal_parse_of_item__of__parse_of_item));
-            simpl in *.
-            Print height_of_parse_production.
-            refine (let mp1 := (@minimal_parse_of_production__of__parse_of_production0 _ p_small _ valid _ p1' (Max.le_max_r _ _) (snd forall_parse)) in
-                    _).
-            hnf in *.
-SearchAbout max.
-SearchAbout (?x < ?y -> ?y <= ?z -> ?x < ?z).
-SearchAbout (?x <= max _ ?x).
+            simpl in *;
+            try solve [ subst; rewrite ?LeftId, ?RightId; trivial ].
+          Defined.
+        End helper.
 
-
-
- valid valid_map p1' (snd forall_parse) in
-            change (max (S (height_of_parse_item' (@height_of_parse _ _ _) p0'))
-                        (height_of_parse_production p1') < S h') in p_small.
-            SearchAbout (S ?x < ?y -> ?x < ?y).
-            refine () in
-                    _).
-
-          p as p in (parse_of_production _ _ str pat)
-          return
-          (Forall_parse_of_production P p
-           -> minimal_parse_of_production valid str pat + alt_option valid str (@proj1_sig _ _ ∘ valid_map))
-        with
-          | ParseProductionNil
-            => fun _ => inl (MinParseProductionNil _)
-          | ParseProductionCons str0 pat' str1 pats' p0' p1'
-            => fun forall_parse
-               => let mp0 := minimal_parse_of_item__of__parse_of_item' valid valid_map (@minimal_parse_of__of__parse_of) p0' (fst forall_parse) in
-                  let mp1 := minimal_parse_of_production__of__parse_of_production valid valid_map p1' (snd forall_parse) in
-                  let mp0' := alt_all_elim (minimal_parse_of_item__of__parse_of_item' initial_productions_data (fun _ => None) (@minimal_parse_of__of__parse_of) p0' (fst forall_parse)) in
-                  let mp1' := alt_all_elim (minimal_parse_of_production__of__parse_of_production initial_productions_data (fun _ => None) p1' (snd forall_parse)) in
-
-
-                  match stringlike_dec str0 (Empty _), stringlike_dec str1 (Empty _) with
-                    | right pf0, right pf1
-                      => inl (MinParseProductionConsDec valid pf0 pf1 admit (*mp0'*) mp1')
-                    | left pf0, left pf1
-                      => let eq_pf0 := (_ : str0 = str0 ++ str1) in
-                         let eq_pf1 := (_ : str1 = str0 ++ str1) in
-                         match mp0, mp1 with
-                           | inl mp0'', inl mp1''
-                             => inl (MinParseProductionConsEmpty01 pf0 pf1 mp0'' mp1'')
-                           | inr other, _
-                             => inr (match eq_pf0 in (_ = str1) return (alt_option valid str1 (@proj1_sig _ _ ∘ valid_map)) with
-                                       | eq_refl => other
-                                     end)
-                           | _, inr other
-                             => inr (match eq_pf1 in (_ = str1) return (alt_option valid str1 (@proj1_sig _ _ ∘ valid_map)) with
-                                       | eq_refl => other
-                                     end)
-                         end
-                    | left pf0, right pf1
-                      => let eq_pf := (_ : str1 = str0 ++ str1) in
-                         match mp1 with
-                           | inl mp1''
-                             => inl (MinParseProductionConsEmpty0 pf0 pf1 _(*mp0'*) mp1'')
-                           | inr other
-                             => inr (match eq_pf in (_ = str0) return (alt_option valid str0 (@proj1_sig _ _ ∘ valid_map)) with
-                                       | eq_refl => other
-                                     end)
-                         end
-                    | right pf0, left pf1
-                      => let eq_pf := (_ : str0 = str0 ++ str1) in
-                         _ (*match mp0 with
-                           | inl mp0''
-                             => inl (MinParseProductionConsEmpty1 pf0 pf1 mp0'' mp1')
-                           | inr other
-                             => inr (match eq_pf in (_ = str0) return (alt_option valid str0) with
-                                       | eq_refl => other
-                                     end)
-                         end*)
-                  end
-        end.
-
-      minimal_parse_of_production__of__parse_of_production
-             {str : String} (valid : productions_listT) {pat : production CharType}
-             (valid_map : valid_mapT)
-             (p : parse_of_production String G str pat)
-             {struct p}
-    : Forall_parse_of_production P p -> (minimal_parse_of_production valid str pat + alt_option valid str (@proj1_sig _ _ ∘ valid_map))
-      := match
-          p as p in (parse_of_production _ _ str pat)
-          return
-          (Forall_parse_of_production P p
-           -> minimal_parse_of_production valid str pat + alt_option valid str (@proj1_sig _ _ ∘ valid_map))
-        with
-          | ParseProductionNil
-            => fun _ => inl (MinParseProductionNil _)
-          | ParseProductionCons str0 pat' str1 pats' p0' p1'
-            => fun forall_parse
-               => let mp0 := minimal_parse_of_item__of__parse_of_item' valid valid_map (@minimal_parse_of__of__parse_of) p0' (fst forall_parse) in
-                  let mp1 := minimal_parse_of_production__of__parse_of_production valid valid_map p1' (snd forall_parse) in
-                  let mp0' := alt_all_elim (minimal_parse_of_item__of__parse_of_item' initial_productions_data (fun _ => None) (@minimal_parse_of__of__parse_of) p0' (fst forall_parse)) in
-                  let mp1' := alt_all_elim (minimal_parse_of_production__of__parse_of_production initial_productions_data (fun _ => None) p1' (snd forall_parse)) in
-
-
-                  match stringlike_dec str0 (Empty _), stringlike_dec str1 (Empty _) with
-                    | right pf0, right pf1
-                      => inl (MinParseProductionConsDec valid pf0 pf1 admit (*mp0'*) mp1')
-                    | left pf0, left pf1
-                      => let eq_pf0 := (_ : str0 = str0 ++ str1) in
-                         let eq_pf1 := (_ : str1 = str0 ++ str1) in
-                         match mp0, mp1 with
-                           | inl mp0'', inl mp1''
-                             => inl (MinParseProductionConsEmpty01 pf0 pf1 mp0'' mp1'')
-                           | inr other, _
-                             => inr (match eq_pf0 in (_ = str1) return (alt_option valid str1 (@proj1_sig _ _ ∘ valid_map)) with
-                                       | eq_refl => other
-                                     end)
-                           | _, inr other
-                             => inr (match eq_pf1 in (_ = str1) return (alt_option valid str1 (@proj1_sig _ _ ∘ valid_map)) with
-                                       | eq_refl => other
-                                     end)
-                         end
-                    | left pf0, right pf1
-                      => let eq_pf := (_ : str1 = str0 ++ str1) in
-                         match mp1 with
-                           | inl mp1''
-                             => inl (MinParseProductionConsEmpty0 pf0 pf1 _(*mp0'*) mp1'')
-                           | inr other
-                             => inr (match eq_pf in (_ = str0) return (alt_option valid str0 (@proj1_sig _ _ ∘ valid_map)) with
-                                       | eq_refl => other
-                                     end)
-                         end
-                    | right pf0, left pf1
-                      => let eq_pf := (_ : str0 = str0 ++ str1) in
-                         _ (*match mp0 with
-                           | inl mp0''
-                             => inl (MinParseProductionConsEmpty1 pf0 pf1 mp0'' mp1')
-                           | inr other
-                             => inr (match eq_pf in (_ = str0) return (alt_option valid str0) with
-                                       | eq_refl => other
-                                     end)
-                         end*)
-                  end
-        end.
-
-    Local Obligation Tactic := program_simpl; rewrite ?LeftId, ?RightId; trivial.
-
-    Program Fixpoint minimal_parse_of__of__parse_of
-             {str : String} (valid : productions_listT) {pats : productions CharType}
-             (valid_map : valid_mapT)
-             (p : parse_of String G str pats)
-             {struct p}
-    : Forall_parse_of P p -> (minimal_parse_of valid str pats + alt_option valid str (@proj1_sig _ _ ∘ valid_map))
-      := match
-          p as p in (parse_of _ _ str pats)
-          return
-          (Forall_parse_of P p
-           -> minimal_parse_of valid str pats + alt_option valid str (@proj1_sig _ _ ∘ valid_map))
-        with
-          | ParseHead _ pat' pats' p'
-            => fun forall_parse
-               => match minimal_parse_of_production__of__parse_of_production valid valid_map p' forall_parse with
-                    | inl mp => inl (MinParseHead pats' mp)
-                    | inr other => inr other
-                  end
-          | ParseTail _ pat' pats' p'
-            => fun forall_parse
-               => match minimal_parse_of__of__parse_of valid valid_map p' forall_parse with
-                    | inl mp => inl (MinParseTail pat' mp)
-                    | inr other => inr other
-                  end
-        end
-    with minimal_parse_of_production__of__parse_of_production
-             {str : String} (valid : productions_listT) {pat : production CharType}
-             (valid_map : valid_mapT)
-             (p : parse_of_production String G str pat)
-             {struct p}
-    : Forall_parse_of_production P p -> (minimal_parse_of_production valid str pat + alt_option valid str (@proj1_sig _ _ ∘ valid_map))
-      := match
-          p as p in (parse_of_production _ _ str pat)
-          return
-          (Forall_parse_of_production P p
-           -> minimal_parse_of_production valid str pat + alt_option valid str (@proj1_sig _ _ ∘ valid_map))
-        with
-          | ParseProductionNil
-            => fun _ => inl (MinParseProductionNil _)
-          | ParseProductionCons str0 pat' str1 pats' p0' p1'
-            => fun forall_parse
-               => let mp0 := minimal_parse_of_item__of__parse_of_item' valid valid_map (@minimal_parse_of__of__parse_of) p0' (fst forall_parse) in
-                  let mp1 := minimal_parse_of_production__of__parse_of_production valid valid_map p1' (snd forall_parse) in
-                  let mp0' := alt_all_elim (minimal_parse_of_item__of__parse_of_item' initial_productions_data (fun _ => None) (@minimal_parse_of__of__parse_of) p0' (fst forall_parse)) in
-                  let mp1' := alt_all_elim (minimal_parse_of_production__of__parse_of_production initial_productions_data (fun _ => None) p1' (snd forall_parse)) in
-
-
-                  match stringlike_dec str0 (Empty _), stringlike_dec str1 (Empty _) with
-                    | right pf0, right pf1
-                      => inl (MinParseProductionConsDec valid pf0 pf1 admit (*mp0'*) mp1')
-                    | left pf0, left pf1
-                      => let eq_pf0 := (_ : str0 = str0 ++ str1) in
-                         let eq_pf1 := (_ : str1 = str0 ++ str1) in
-                         match mp0, mp1 with
-                           | inl mp0'', inl mp1''
-                             => inl (MinParseProductionConsEmpty01 pf0 pf1 mp0'' mp1'')
-                           | inr other, _
-                             => inr (match eq_pf0 in (_ = str1) return (alt_option valid str1 (@proj1_sig _ _ ∘ valid_map)) with
-                                       | eq_refl => other
-                                     end)
-                           | _, inr other
-                             => inr (match eq_pf1 in (_ = str1) return (alt_option valid str1 (@proj1_sig _ _ ∘ valid_map)) with
-                                       | eq_refl => other
-                                     end)
-                         end
-                    | left pf0, right pf1
-                      => let eq_pf := (_ : str1 = str0 ++ str1) in
-                         match mp1 with
-                           | inl mp1''
-                             => inl (MinParseProductionConsEmpty0 pf0 pf1 _(*mp0'*) mp1'')
-                           | inr other
-                             => inr (match eq_pf in (_ = str0) return (alt_option valid str0 (@proj1_sig _ _ ∘ valid_map)) with
-                                       | eq_refl => other
-                                     end)
-                         end
-                    | right pf0, left pf1
-                      => let eq_pf := (_ : str0 = str0 ++ str1) in
-                         _ (*match mp0 with
-                           | inl mp0''
-                             => inl (MinParseProductionConsEmpty1 pf0 pf1 mp0'' mp1')
-                           | inr other
-                             => inr (match eq_pf in (_ = str0) return (alt_option valid str0) with
-                                       | eq_refl => other
-                                     end)
-                         end*)
-                  end
-        end.
-    Obligation 1 of minimal_parse_of_production__of__parse_of_production.
-    Axiom forall_extensionality : forall {A P P'}, (forall x : A, P x = P' x) -> (forall x, P x) = (forall x, P' x).
-    Unset Printing All.
-
-    repeat (apply forall_extensionality; intro).
-    repeat match goal with
-             | [ |- (forall x : ?T, @?P x) = (forall x : ?T, @?P' x) ]
-               => apply (@forall_extensionality T P P'); intro
-             | _ => progress f_equal; []
-             | _ => apply functional_extensionality_dep; intro
-           end.
-    repeat (
-    .
-    apply forall_extensionality.
-    admit.
-    Defined.
-    Obligation 2 of minimal_parse_of_production__of__parse_of_production.
-
-
-    eapply alt_all_elim in x1.
-    pose .
-                    ()
-    (minimal_parse_of_production__of__parse_of_production _ p1' (snd forall_parse)))
-    MinParseProductionConsDec
-
-                 | left pf,
-                   => match pf in (_ = str0)
-                            return (forall p0'' : parse_of_item String G str0 pat',
-                                      (Forall_parse_of_item P p0'' *
-                                       Forall_parse_of_production P p1')%type
-                                      -> minimal_parse_of_production valid (str0 ++ str1) (pat'::pats') + _)
-                      with
-                        | eq_refl
-                          => fun p0'' forall_parse
-                             => inl (MinParseProductionConsEmpty0
-                                       _
-                                       (minimal_parse_of_production__of__parse_of_production _ p1' (snd forall_parse)))
-                      end p0'
-                 | right pf => _
-               end
-        end.
-    Obligation 1 of minimal_parse_of_production__of__parse_of_production.
-
-    pose (
-
-            => match stringlike_dec (Empty _) str0 with
-                 | left pf
-                   => match pf in (_ = str0)
-                            return (forall p0'' : parse_of_item String G str0 pat',
-                                      (Forall_parse_of_item P p0'' *
-                                       Forall_parse_of_production P p1')%type
-                                      -> minimal_parse_of_production valid (str0 ++ str1) (pat'::pats') + _)
-                      with
-                        | eq_refl
-                          => fun p0'' forall_parse
-                             => inl (MinParseProductionConsEmpty0
-                                       _
-                                       (minimal_parse_of_production__of__parse_of_production _ p1' (snd forall_parse)))
-                      end p0'
-                 | right pf => _
-               end
-        end.
-    Obligation 1 of minimal_parse_of_production__of__parse_of_production.
-    simpl in *.
-    Print Forall_parse_of_production.
-Show Proof.
-
-    pose (minimal_parse_of_production__of__parse_of_production valid p' forall_parse).
-      Show Proof.
-
-      constructor.
-      Show Proof.
-
-      destruct p.
-      Show Proof.
-
-
-    Next Obligation.
-    with
-
-    Proof.
-
-                                         + { p' : _ & (is_valid_productions valid p' = false /\ P p')
-                                                      * minimal_parse_of initial_productions_data str p' })%type
-           {
-      Print Forall_parse_of.
-
-      unfold Forall_parse_of in *.
-      fold Forall_parse_of in *.
-      simpl in *.
-      Print Forall_parse_of.
-      hnf in forall_parse.
-      inversion forall_parse.
-    destruct p.
-    Show Proof.
-    Proof.
-      destruct p.
-             (p : productions
-             {str valid}
-
-
-
-    Section parts.
-      Local Hint Constructors parse_of_item parse_of parse_of_production.
-      Local Hint Constructors minimal_parse_of_item minimal_parse_of minimal_parse_of_production.
-
-
-
-: forall valid x,
-                                                    minimal_parse_of_item valid [[ x ]]%string_like (Terminal x)
-                   |
-
-forall valid name str,
-                              is_valid_productions valid (Lookup G name) = true
-                              -> minimal_parse_of (remove_productions valid (Lookup G name)) str (Lookup G name)
-                              -> minimal_parse_of_item valid str (NonTerminal CharType name).
-
-(remove_productions valid (Lookup G name))
-
-        is_valid_productions valid (Lookup G name) = true
-        -> minimal_parse_of (remove_productions valid (Lookup G name)) str (Lookup G name)
-        -> minimal_parse_of_item valid str (NonTerminal CharType name).
-
-
-        (** We require that the list of productions be non-empty; we
-            do this by passing the first element separately, rather
-            than invoking dependent types and proofs. *)
-        Context (str : String)
-                (str_matches_productions : production CharType -> productions CharType -> bool).
-
-        Definition parse_item (it : item CharType) : bool
-          := match it with
-               | Terminal ch => [[ ch ]] =s str
-               | NonTerminal name => match Lookup G name with
-                                       | nil => (** No string can match an empty nonterminal *) false
-                                       | p::ps => str_matches_productions p ps
-                                     end
-             end.
-      End item.
-(*match productions_dec chartype_dec (G name) (G name') as s1
-                                               return
-                                               (_ * minimal_parse_of (remove_productions (` (match s1 with
-                                                                                               | left pf => match pf in (_ = y) return {v : productions_listT | is_valid_productions v y = true} with
-                                                                                                              | eq_refl => exist _ valid H'
-                                                                                                            end
-                                                                                               | right _ => valid_map name'
-                                                                                             end)) _) _ _ -> _)
-                                         with
-                                           | left e
-                                             => fun other
-                                                => let f := fun p
-                                                            => (match e as e in (_ = y)
-                                                                      return
-                                                                      ((is_valid_productions _ y = false /\ P y) *
-                                                                       minimal_parse_of
-                                                                         (remove_productions
-                                                                            (proj1_sig (match e in (_ = y) return {v : productions_listT | is_valid_productions v y = true} with
-                                                                                          | eq_refl => _
-                                                                                        end)) y) str' y
-                                                                       -> minimal_parse_of_item valid str' (NonTerminal CharType name) +
-                                                                          alt_option valid str' (@proj1_sig _ _ ∘ valid_map))
-                                                                with
-                                                                  | eq_refl
-                                                                    => fun other
-                                                                       => inl (MinParseNonTerminal name H' (p other))
-                                                                end other) in
-                                                   f (@snd _ _)
-                                           | right n =>
-                                             fun other
-                                             => inr (existT _ name' (conj (match proj1 (remove_productions_2 _ _ _) (proj1 (fst other)) with
-                                                                             | or_introl H' => H'
-                                                                             | or_intror H' => match n H' : False with end
-                                                                           end) (proj2 (fst other)),
-                                                                     (snd other)))
-                                         end other*)
-
-      Section item.
-
-
-        Context (str : String)
-                (str_matches_productions : production CharType -> productions CharType -> bool).
-
-
-  | MinParseTerminal : forall valid x,
-                         minimal_parse_of_item valid [[ x ]]%string_like (Terminal x)
-  | MinParseNonTerminal
-    : forall valid name str,
-        is_valid_productions valid (Lookup G name) = true
-        -> minimal_parse_of (remove_productions valid (Lookup G name)) str (Lookup G name)
-        -> minimal_parse_of_item valid str (NonTerminal CharType name).
-
-        Definition str_matches_productions_soundT
-          := forall prod prods, str_matches_productions prod prods = true
-                                -> parse_of _ G str (prod::prods).
-
-        Definition str_matches_productions_completeT
-          := forall prod prods, parse_of _ G str (prod::prods)
-                                -> str_matches_productions prod prods = true.
-
-        Lemma parse_item_sound
-              (str_matches_productions_sound : str_matches_productions_soundT)
-              (it : item CharType)
-        : parse_item String G str str_matches_productions it = true -> parse_of_item _ G str it.
-        Proof.
-          unfold parse_item, str_matches_productions_soundT in *.
-          repeat match goal with
-                   | _ => intro
-                   | [ H : context[match ?E with _ => _ end] |- _ ] => atomic E; destruct E
-                   | [ |- context[match ?E with _ => _ end] ] => atomic E; destruct E
-                   | [ H : _ = true |- _ ] => apply bool_eq_correct in H
-                   | [ |- parse_of_item _ _ _ (NonTerminal _ _) ] => constructor
-                   | [ H : context[match ?E with _ => _ end] |- context[?E] ] => destruct E
-                   | _ => progress subst
-                   | _ => solve [ eauto ]
-                 end.
-        Defined.
-
-        Lemma parse_item_complete
-              (str_matches_productions_complete : str_matches_productions_completeT)
-              (it : item CharType)
-        : parse_of_item _ G str it -> parse_item String G str str_matches_productions it = true.
-        Proof.
-          unfold parse_item, str_matches_productions_completeT in *.
-          repeat match goal with
-                   | _ => intro
-                   | _ => reflexivity
-                   | [ H : parse_of_item _ _ ?s ?i |- _ ] => atomic s; atomic i; destruct H
-                   | [ |- _ = true ] => apply bool_eq_correct
-                   | [ H : context[?E] |- context[match ?E with _ => _ end] ] => destruct E
-                   | [ H : parse_of _ _ _ [] |- _ ] => solve [ inversion H ]
-                   | _ => solve [ eauto ]
-               end.
-        Qed.
-      End item.
-
-      Section item_ext.
-        Lemma parse_item_ext
-              (str : String)
-              (str_matches_productions1 str_matches_productions2 : production CharType -> productions CharType -> bool)
-              (it : item CharType)
-              (ext : forall x y, str_matches_productions1 x y = str_matches_productions2 x y)
-        : parse_item String G str str_matches_productions1 it
-          = parse_item String G str str_matches_productions2 it.
-        Proof.
-          unfold parse_item.
-          destruct it; auto;
-          match goal with
-            | [ |- context[match ?E with _ => _ end] ] => destruct E
-          end;
-          auto.
-        Qed.
-      End item_ext.
-
-      Section production.
-        Context (str0 : String)
-                (parse_productions : forall (str : String),
-                                       str ≤s str0
-                                       -> production CharType
-                                       -> productions CharType
-                                       -> bool).
-
-        Definition parse_productions_soundT
-          := forall str pf prod prods,
-               @parse_productions str pf prod prods = true
-               -> parse_of _ G str (prod::prods).
-
-        Definition parse_productions_completeT
-          := forall str pf prod prods,
-               parse_of _ G str (prod::prods)
-               -> @parse_productions str pf prod prods = true.
-
-        Definition split_correctT
-                   (str1 : String)
-                   (split : String * String)
-          := fst split ++ snd split =s str1.
-
-        Definition split_list_correctT str1 (split_list : list (String * String))
-          := List.Forall (@split_correctT str1) split_list.
-
-        Definition split_list_completeT
-                   (str : String) (pf : str ≤s str0)
-                   (split_list : list (String * String))
-                   (prod : production CharType)
-          := match prod return Type with
-               | nil => True
-               | it::its => ({ s1s2 : String * String
-                                      & (fst s1s2 ++ snd s1s2 =s str)
-                                        * (parse_of_item _ G (fst s1s2) it)
-                                        * (parse_of_production _ G (snd s1s2) its) }%type)
-                            -> ({ s1s2 : String * String
-                                         & (In s1s2 split_list)
-                                           * (parse_of_item _ G (fst s1s2) it)
-                                           * (parse_of_production _ G (snd s1s2) its) }%type)
-             end.
-
-        Lemma parse_production_sound
-                 (parse_productions_sound : parse_productions_soundT)
-                 (str : String) (pf : str ≤s str0)
-                 (prod : production CharType)
-        : parse_production G split_string_for_production split_string_for_production_correct parse_productions pf prod = true
-          -> parse_of_production _ G str prod.
-        Proof.
-          change (forall str0 prod, split_list_correctT str0 (split_string_for_production str0 prod)) in split_string_for_production_correct.
-          revert str pf; induction prod;
-          repeat match goal with
-                   | _ => intro
-                   | _ => progress simpl in *
-                   | _ => progress subst
-                   | _ => solve [ auto ]
-                   | [ H : fold_right orb false (map _ _) = true |- _ ] => apply fold_right_orb_map_sig1 in H
-                   | [ H : (_ || _)%bool = true |- _ ] => apply Bool.orb_true_elim in H
-                   | [ H : (_ && _)%bool = true |- _ ] => apply Bool.andb_true_iff in H
-                   | _ => progress destruct_head sumbool
-                   | _ => progress destruct_head and
-                   | _ => progress destruct_head sig
-                   | _ => progress simpl in *
-                   | _ => progress subst
-                   | [ H : (_ =s _) = true |- _ ] => apply bool_eq_correct in H
-                   | [ H : (_ =s _) = true |- _ ]
-                     => let H' := fresh in
-                        pose proof H as H';
-                          apply bool_eq_correct in H';
-                          progress subst
-                 end.
-          { constructor;
-            solve [ eapply IHprod; eassumption
-                  | eapply parse_item_sound; try eassumption;
-                    hnf in parse_productions_sound |- *;
-                    apply parse_productions_sound ]. }
-        Defined.
-
-        Lemma parse_production_complete
-                 (parse_productions_complete : parse_productions_completeT)
-                 (split_string_for_production_complete : forall str pf prod, @split_list_completeT str pf (split_string_for_production str prod) prod)
-                 (str : String) (pf : str ≤s str0)
-                 (prod : production CharType)
-        : parse_of_production _ G str prod
-          -> parse_production G split_string_for_production split_string_for_production_correct parse_productions pf prod = true.
-        Proof.
-          change (forall str0 prod, split_list_correctT str0 (split_string_for_production str0 prod)) in split_string_for_production_correct.
-          revert str pf; induction prod;
-          repeat match goal with
-                   | _ => intro
-                   | _ => progress simpl in *
-                   | _ => progress subst
-                   | _ => solve [ auto ]
-                   | [ H : fold_right orb false (map _ _) = true |- _ ] => apply fold_right_orb_map_sig1 in H
-                   | [ H : (_ || _)%bool = true |- _ ] => apply Bool.orb_true_elim in H
-                   | [ H : (_ && _)%bool = true |- _ ] => apply Bool.andb_true_iff in H
-                   | [ H : parse_of_production _ _ _ nil |- _ ] => inversion_clear H
-                   | [ |- (_ =s _) = true ] => apply bool_eq_correct
-                   | _ => progress destruct_head_hnf sumbool
-                   | _ => progress destruct_head_hnf and
-                   | _ => progress destruct_head_hnf sig
-                   | _ => progress destruct_head_hnf sigT
-                   | _ => progress destruct_head_hnf Datatypes.prod
-                   | _ => progress simpl in *
-                   | _ => progress subst
-                   | [ H : (_ =s _) = true |- _ ] => apply bool_eq_correct in H
-                   | [ H : (_ =s _) = true |- _ ]
-                     => let H' := fresh in
-                        pose proof H as H';
-                          apply bool_eq_correct in H';
-                          progress subst
-                   | [ H : parse_of_production _ _ _ (_::_) |- _ ] => inversion H; clear H; subst
-                   | [ H : ?s ≤s _ |- context[split_string_for_production_correct ?s ?p] ]
-                     => specialize (fun a b p0 p1 p2
-                                    => @split_string_for_production_complete s H p (existT _ (a, b) (p0, p1, p2)))
-                   | [ H : forall a b, is_true (a ++ b =s _ ++ _) -> _ |- _ ]
-                     => specialize (H _ _ (proj2 (@bool_eq_correct _ _ _ _) eq_refl))
-                   | [ H : ?a -> ?b, H' : ?a |- _ ] => specialize (H H')
-                   | [ |- fold_right orb false (map _ _) = true ] => apply fold_right_orb_map_sig2
-                 end.
-          match goal with
-            | [ H : In (?s1, ?s2) (split_string_for_production ?str ?prod)
-                |- { x : { s1s2 : _ | (fst s1s2 ++ snd s1s2 =s ?str) = true } | _ } ]
-              => let H' := fresh in
-                 pose proof (proj1 (@Forall_forall _ _ _) (@split_string_for_production_correct str prod) _ H) as H';
-                   unfold split_correctT in H';
-                   refine (exist _ (exist _ (s1, s2) _) _);
-                   simpl in *
-          end.
-          repeat match goal with
-                   | _ => split
-                   | [ |- (_ && _)%bool = true ] => apply Bool.andb_true_iff
-                   | _ => eapply parse_item_complete; try eassumption;
-                          hnf in parse_productions_complete |- *;
-                          solve [ apply parse_productions_complete ]
-                   | _ => eapply IHprod; eassumption
-                 end.
-          apply In_combine_sig.
-          Grab Existential Variables.
-          assumption.
-        Qed.
+        Definition minimal_parse_of_production__of__parse_of_production'
+        : forall (h : nat)
+                 (minimal_parse_of__of__parse_of : of_parse_T h)
+                 {str} valid {pat}
+                 (p : parse_of_production String G str pat),
+            @of_parse_production_T str valid pat p h
+          := Fix Wf_nat.lt_wf _ minimal_parse_of_production__of__parse_of_production'_helper.
       End production.
 
-      Section production_ext.
-        Lemma parse_production_ext
-              (str0 : String)
-              (parse_productions1 parse_productions2 : forall (str : String),
-                                                         str ≤s str0
-                                                         -> production CharType
-                                                         -> productions CharType
-                                                         -> bool)
-              (str : String) (pf : str ≤s str0) (prod : production CharType)
-              (ext : forall str' pf' prod' prods', parse_productions1 str' pf' prod' prods'
-                                                   = parse_productions2 str' pf' prod' prods')
-        : parse_production G split_string_for_production split_string_for_production_correct parse_productions1 pf prod
-          = parse_production G split_string_for_production split_string_for_production_correct parse_productions2 pf prod.
-        Proof.
-          revert str pf.
-          induction prod as [|? ? IHprod]; simpl; intros; try reflexivity; [].
-          f_equal.
-          apply map_ext; intros.
-          apply f_equal2; [ apply parse_item_ext | apply IHprod ].
-          intros; apply ext.
-        Qed.
-      End production_ext.
+      Section parse_of.
+        Let rec_T h
+          := forall h', h' < h -> of_parse_T h'.
 
-      Section productions.
-        Section step.
-          Variable str0 : String.
-          Variable parse_productions : forall (str : String)
-                                              (pf : str ≤s str0),
-                                         production CharType -> productions CharType -> bool.
+        Section helper.
+          Context (h : nat)
+                  (minimal_parse_of__of__parse_of_rec : rec_T h).
 
-          Local Ltac parse_productions_step_t :=
-            repeat match goal with
-                     | _ => intro
-                     | [ H : (_ || _)%bool = true |- _ ] => apply Bool.orb_true_elim in H
-                     | [ H : (_ && _)%bool = true |- _ ] => apply Bool.andb_true_iff in H
-                     | [ |- (_ || _)%bool = true ] => apply Bool.orb_true_iff
-                     | [ |- (_ =s _) = true ] => apply bool_eq_correct
-                     | [ H : (_ =s _) = true |- _ ] => apply bool_eq_correct in H
-                     | _ => progress destruct_head_hnf sumbool
-                     | _ => progress destruct_head_hnf and
-                     | _ => progress destruct_head_hnf sig
-                     | _ => progress destruct_head_hnf sigT
-                     | _ => progress destruct_head_hnf Datatypes.prod
-                     | _ => progress simpl in *
-                     | _ => progress subst
-                     | [ H : parse_of _ _ _ nil |- _ ] => solve [ inversion H ]
-                     | [ H : parse_of _ _ _ (_::_) |- _ ] => inversion H; clear H; subst
-                     | [ H : parse_production _ _ _ _ _ _ = true |- _ ] => apply parse_production_sound in H; try eassumption; []
-                     | _ => solve [ eauto ]
-                   end.
+          Let minimal_parse_of__of__parse_of h' H
+          : of_parse_T h'
+            := @minimal_parse_of__of__parse_of_rec h' H.
 
+          Context {str : String} (valid : productions_listT) {pats : productions CharType}.
 
-          (** To parse as a given list of [production]s, we must parse as one of the [production]s. *)
-          Lemma parse_productions_step_sound
-                (parse_productions_sound : parse_productions_soundT parse_productions)
-                (str : String) (pf : str ≤s str0) (prod : production CharType) (prods : productions CharType)
-          : parse_productions_step G split_string_for_production split_string_for_production_correct parse_productions pf (prod::prods) = true
-            -> parse_of _ G str (prod::prods).
-          Proof.
-            unfold parse_productions_step.
-            revert prod.
-            induction prods; simpl; auto; intros.
-            { parse_productions_step_t. }
-            { parse_productions_step_t.
-              apply ParseTail.
-              apply IHprods; clear IHprods.
-              parse_productions_step_t. }
-          Defined.
+          Definition minimal_parse_of__of__parse_of'_helper
+                     (p : parse_of String G str pats)
+          : @of_parse_T' h str valid pats p
+            := match h as h, p as p in (parse_of _ _ str pats)
+                     return ((forall h' (H : h' < h), of_parse_T h')
+                             -> @of_parse_T' h str valid pats p)
+               with
+                 | 0, _ => fun _ H' => match Lt.lt_n_0 _ H' : False with end
+                 | S h', ParseHead _ pat' pats' p'
+                   => fun minimal_parse_of__of__parse_of
+                          p_small
+                          forall_parse
+                      => let minimal_parse_of_production__of__parse_of_production
+                               {str} valid {pat}
+                             := @minimal_parse_of_production__of__parse_of_production' h' (@minimal_parse_of__of__parse_of _ (Lt.lt_n_Sn _)) str valid pat in
+                         match minimal_parse_of_production__of__parse_of_production valid p' (Lt.lt_S_n _ _ p_small) forall_parse with
+                           | inl mp
+                             => inl (existT
+                                       _ (MinParseHead pats' (projT1 mp))
+                                       (Le.le_n_S _ _ (fst (projT2 mp)),
+                                        snd (projT2 mp)))
+                           | inr other
+                             => inr (expand_alt_option
+                                       (Lt.lt_n_Sn _)
+                                       (reflexivity _)
+                                       (reflexivity _)
+                                       other)
+                         end
+                 | S h', ParseTail _ pat' pats' p'
+                   => fun minimal_parse_of__of__parse_of
+                          p_small
+                          forall_parse
+                      => match minimal_parse_of__of__parse_of _ (Lt.lt_n_Sn _) _ valid _ p' (Lt.lt_S_n _ _ p_small) forall_parse with
+                           | inl mp
+                             => inl (existT
+                                       _ (MinParseTail pat' (projT1 mp))
+                                       (Le.le_n_S _ _ (fst (projT2 mp)),
+                                        snd (projT2 mp)))
+                           | inr other
+                             => inr (expand_alt_option
+                                       (Lt.lt_n_Sn _)
+                                       (reflexivity _)
+                                       (reflexivity _)
+                                       other)
+                         end
+               end
+                 (@minimal_parse_of__of__parse_of).
+        End helper.
 
-          Lemma parse_productions_step_complete
-                (parse_productions_complete : parse_productions_completeT parse_productions)
-                (split_string_for_production_complete : forall str pf prod, @split_list_completeT str0 str pf (split_string_for_production str prod) prod)
-                (str : String) (pf : str ≤s str0) (prod : production CharType) (prods : productions CharType)
-          : parse_of _ G str (prod::prods)
-            -> parse_productions_step G split_string_for_production split_string_for_production_correct parse_productions pf (prod::prods) = true.
-          Proof.
-            unfold parse_productions_step.
-            revert prod.
-            induction prods; simpl; auto.
-            { parse_productions_step_t.
-              left; apply parse_production_complete; assumption. }
-            { parse_productions_step_t.
-              match goal with
-                | [ H : forall prod, parse_of _ _ ?s (prod::_) -> _,
-                      H' : parse_of_production _ _ ?s ?prod |- _ ]
-                  => specialize (H prod (ParseHead _ H'))
-              end.
-              parse_productions_step_t.
-              right.
-              parse_productions_step_t. }
-          Qed.
-        End step.
+        Definition minimal_parse_of__of__parse_of'
+        : forall (h : nat)
+                 {str} valid {pats}
+                 (p : parse_of String G str pats),
+            @of_parse_T' h str valid pats p
+          := Fix Wf_nat.lt_wf _ minimal_parse_of__of__parse_of'_helper.
+      End parse_of.
+    End wf_parts.
 
-        Section step_extensional.
-          Lemma parse_productions_step_ext (str0 : String)
-                (parse_productions1 parse_productions2 : forall (str : String)
-                                                                (pf : str ≤s str0),
-                                                           production CharType -> productions CharType -> bool)
-                (str : String) (pf : str ≤s str0) (prods : productions CharType)
-                (ext : forall str' pf' prod' prods', parse_productions1 str' pf' prod' prods'
-                                                     = parse_productions2 str' pf' prod' prods')
-          : parse_productions_step G split_string_for_production split_string_for_production_correct parse_productions1 pf prods
-            = parse_productions_step G split_string_for_production split_string_for_production_correct parse_productions2 pf prods.
-          Proof.
-            unfold parse_productions_step.
-            f_equal.
-            apply map_ext; intros.
-            apply parse_production_ext; auto.
-          Qed.
-        End step_extensional.
+    Definition minimal_parse_of__of__parse_of
+               {str : String} {pats : productions CharType}
+               (p : parse_of String G str pats)
+               (H : Forall_parse_of P p)
+    : minimal_parse_of initial_productions_data str pats
+      := match @minimal_parse_of__of__parse_of'
+                 _ str initial_productions_data pats p
+                 (Lt.lt_n_Sn _)
+                 H with
+           | inl p' => projT1 p'
+           | inr other => let H' := fst (projT2 other) in
+                          match Bool.eq_true_false_abs _ (proj2 H') (proj1 H') : False with end
+         end.
 
-        (** TODO: move this elsewhere *)
-        Lemma or_to_sumbool (s1 s2 : String) (f : String -> nat)
-              (H : f s1 < f s2 \/ s1 = s2)
-        : {f s1 < f s2} + {s1 = s2}.
-        Proof.
-          case_eq (s1 =s s2).
-          { intro H'; right; apply bool_eq_correct in H'; exact H'. }
-          { intro H'; left; destruct H; trivial.
-            apply bool_eq_correct in H.
-            generalize dependent (s1 =s s2)%string_like; intros; subst.
-            discriminate. }
-        Qed.
+    Definition minimal_parse_of_production__of__parse_of_production
+               {str : String} {pat : production CharType}
+               (p : parse_of_production String G str pat)
+               (H : Forall_parse_of_production P p)
+    : minimal_parse_of_production initial_productions_data str pat
+      := match @minimal_parse_of_production__of__parse_of_production'
+                 _ (@minimal_parse_of__of__parse_of' _) str initial_productions_data pat p
+                 (Lt.lt_n_Sn _)
+                 H with
+           | inl p' => projT1 p'
+           | inr other => let H' := fst (projT2 other) in
+                          match Bool.eq_true_false_abs _ (proj2 H') (proj1 H') : False with end
+         end.
 
-        (** TODO: move this elsewhere *)
-        Lemma if_ext {T} (b : bool) (f1 f2 : b = true -> T true) (g1 g2 : b = false -> T false)
-              (ext_f : forall H, f1 H = f2 H)
-              (ext_g : forall H, g1 H = g2 H)
-        : (if b as b' return (b = b' -> T b') then f1 else g1) eq_refl
-          = (if b as b' return (b = b' -> T b') then f2 else g2) eq_refl.
-        Proof.
-          destruct b; auto.
-        Defined.
-
-        Section wf.
-          Lemma parse_productions_or_abort_helper_sound
-                (p : String * productions_listT) (str : String)
-                (pf : str ≤s fst p)
-                (prod : production CharType)
-                (prods : productions CharType)
-          : parse_productions_or_abort_helper G initial_productions_data is_valid_productions remove_productions
-                                              remove_productions_dec ntl_wf split_string_for_production
-                                              split_string_for_production_correct
-                                              p pf prod prods
-            = true
-            -> parse_of _ G str (prod::prods).
-          Proof.
-            unfold parse_productions_or_abort_helper.
-            revert str pf prod prods.
-            let Acca := match goal with |- context[@Fix4 _ _ _ _ _ _ ?Rwf _ _ ?a _ _ _ _] => constr:(Rwf a) end in
-            induction (Acca) as [? ? IHr];
-              intros str pf prod prods.
-            rewrite Fix4_eq.
-            { match goal with
-                | [ |- context[match lt_dec ?a ?b with _ => _ end] ] => destruct (lt_dec a b) as [Hlt|Hlt]
-              end.
-              { apply parse_productions_step_sound; try assumption; simpl.
-                hnf.
-                intros str0 pf0 prod0 prods0 H'; eapply IHr;
-                try first [ exact H' | eassumption ].
-                left; assumption. }
-              { let ivp := match goal with |- context[is_valid_productions ?x ?y] => constr:(is_valid_productions x y) end in
-                set (ivp' := ivp);
-                  assert (ivp = ivp') by reflexivity;
-                  clearbody ivp';
-                  destruct ivp'; [ | solve [ auto ] ].
-                intros.
-                hnf in pf.
-                apply or_to_sumbool in pf.
-                destruct pf as [ pf | pf ]; [ exfalso; hnf in *; solve [ auto ] | subst ].
-                eapply parse_productions_step_sound; try eassumption.
-                hnf.
-                intros str0 pf0 prod0 prods0 H'; eapply IHr;
-                try first [ exact H' | eassumption ].
-                right; split; trivial; simpl.
-                apply remove_productions_dec; assumption. } }
-            { repeat match goal with
-                       | _ => intro
-                       | _ => reflexivity
-                       | [ |- context[match ?E with _ => _ end] ] => destruct E
-                       | [ H : _ |- _ ] => rewrite H; reflexivity
-                       | _ => apply parse_productions_step_ext; auto
-                       | _ => apply (@if_ext (fun _ => bool)); intros
-                     end. }
-          Defined.
-
-          Lemma parse_productions_or_abort_helper_complete
-                (p : String * productions_listT) (str : String)
-                (split_string_for_production_complete : forall str0 pf prod, @split_list_completeT str str0 pf (split_string_for_production str0 prod) prod)
-                (pf : str ≤s fst p)
-                (prod : production CharType)
-                (prods : productions CharType)
-          : parse_of _ G str (prod::prods)
-            -> parse_productions_or_abort_helper G initial_productions_data is_valid_productions remove_productions
-                                              remove_productions_dec ntl_wf split_string_for_production
-                                              split_string_for_production_correct
-                                              p pf prod prods
-               = true.
-          Proof.
-            unfold parse_productions_or_abort_helper.
-            revert str split_string_for_production_complete pf prod prods.
-            let Acca := match goal with |- context[@Fix4 _ _ _ _ _ _ ?Rwf _ _ ?a _ _ _ _] => constr:(Rwf a) end in
-            induction (Acca) as [? ? IHr];
-              intros str split_string_for_production_complete pf prod prods.
-            rewrite Fix4_eq.
-            { match goal with
-                | [ |- context[if lt_dec ?a ?b then _ else _] ] => destruct (lt_dec a b)
-              end.
-              { apply parse_productions_step_complete; try assumption.
-                hnf.
-                intros str0 pf0 prod0 prods0 H'; eapply IHr;
-                try first [ exact H' | eassumption ].
-                { left; assumption. }
-                { intros; apply split_string_for_production_complete.
-                  etransitivity; eassumption. } }
-              { let ivp := match goal with |- context[is_valid_productions ?x ?y] => constr:(is_valid_productions x y) end in
-                set (ivp' := ivp);
-                  assert (ivp = ivp') by reflexivity;
-                  clearbody ivp';
-                  destruct ivp'.
-                { intros.
-                  hnf in pf.
-                  apply or_to_sumbool in pf.
-                  destruct pf as [ pf | pf ]; [ exfalso; hnf in *; solve [ auto ] | subst ].
-                  eapply parse_productions_step_complete; try eassumption.
-                  hnf.
-                  intros str0 pf0 prod0 prods0 H'; eapply IHr;
-                  try first [ exact H' | eassumption ].
-                  { right; split; trivial; simpl.
-                    apply remove_productions_dec; assumption. }
-                  { intros; apply split_string_for_production_complete.
-                    etransitivity; eassumption. } }
-                { (** INTERESTING CASE HERE - need to show that if not
-                      [is_valid_productions], then we can't have a
-                      parse tree. *)
-                  exfalso; clear; admit. } } }
-            { repeat match goal with
-                       | _ => intro
-                       | _ => reflexivity
-                       | [ |- context[match ?E with _ => _ end] ] => destruct E
-                       | [ H : _ |- _ ] => rewrite H; reflexivity
-                       | _ => apply parse_productions_step_ext; auto
-                       | _ => apply (@if_ext (fun _ => bool)); intros
-                     end. }
-          Defined.
-
-          Lemma parse_productions_sound
-                (str : String) (prods : productions CharType)
-          : parse_productions _ G initial_productions_data is_valid_productions remove_productions
-                              remove_productions_dec ntl_wf split_string_for_production
-                              split_string_for_production_correct
-                              str prods
-            = true
-            -> parse_of _ G str prods.
-          Proof.
-            unfold parse_productions, parse_productions_or_abort.
-            destruct prods; [ solve [ auto ] | ].
-            apply parse_productions_or_abort_helper_sound.
-          Defined.
-
-          Lemma parse_productions_complete
-                (str : String)
-                (split_string_for_production_complete : forall str0 pf prod, @split_list_completeT str str0 pf (split_string_for_production str0 prod) prod)
-                (prods : productions CharType)
-          : parse_of _ G str prods
-            -> parse_productions _ G initial_productions_data is_valid_productions remove_productions
-                                 remove_productions_dec ntl_wf split_string_for_production
-                                 split_string_for_production_correct
-                                 str prods
-               = true.
-          Proof.
-            unfold parse_productions, parse_productions_or_abort.
-            destruct prods; [ solve [ intro H'; inversion H' ] | ].
-            apply parse_productions_or_abort_helper_complete; try assumption.
-          Defined.
-        End wf.
-      End productions.
-    End parts.
-  End general.
-End sound.
-
-
-  Section i
-
-
-    (** A parse of a string into [productions] is a [production] in
-        that list, together with a list of substrings which cover the
-        original string, each of which is a parse of the relevant
-        component of the [production]. *)
-    Inductive parse_of : String -> productions -> Type :=
-    | ParseHead : forall str pat pats, parse_of_production str pat
-                                       -> parse_of str (pat::pats)
-    | ParseTail : forall str pat pats, parse_of str pats
-                                       -> parse_of str (pat::pats)
-    with parse_of_production : String -> production -> Type :=
-    | ParseProductionNil : parse_of_production (Empty _) nil
-    | ParseProductionCons : forall str pat strs pats,
-                           parse_of_item str pat
-                           -> parse_of_production strs pats
-                           -> parse_of_production (str ++ strs) (pat::pats)
-    with parse_of_item : String -> item -> Type :=
-    | ParseTerminal : forall x, parse_of_item [[ x ]]%string_like (Terminal x)
-    | ParseNonTerminal : forall name str, parse_of str (Lookup G name)
-                                          -> parse_of_item str (NonTerminal name).
-
-    Definition ParseProductionSingleton str it (p : parse_of_item str it) : parse_of_production str [ it ].
-    Proof.
-      rewrite <- (RightId _ str).
-      constructor; assumption || constructor.
-    Defined.
-
-    Definition ParseProductionApp str1 str2 p1 p2 (pop1 : parse_of_production str1 p1) (pop2 : parse_of_production str2 p2)
-    : parse_of_production (str1 ++ str2) (p1 ++ p2)%list.
-    Proof.
-      induction pop1; simpl.
-      { rewrite LeftId; assumption. }
-      { rewrite Associativity.
-        constructor; assumption. }
-    Defined.
-
-    Definition ParseApp str1 str2 p1 p2 (po1 : parse_of str1 [ p1 ]) (po2 : parse_of str2 [ p2 ])
-    : parse_of (str1 ++ str2) [ (p1 ++ p2)%list ].
-    Proof.
-      inversion_clear po1; inversion_clear po2;
-      try match goal with
-            | [ H : parse_of _ [] |- _ ] => exfalso; revert H; clear; intro H; abstract inversion H
-          end.
-      { constructor. apply ParseProductionApp; assumption. }
-    Defined.
-  End parse.
-
-  Definition parse_of_grammar (String : string_like CharType) (str : String) (G : grammar) :=
-    parse_of String G str G.
-
-
-  Section definitions.
-    (** An [item] is the basic building block of a context-free
-        grammar; it is either a terminal ([CharType]-literal) or a
-        nonterminal of a given name. *)
-    Inductive item :=
-    | Terminal (_ : CharType)
-    | NonTerminal (name : string).
-
-    (** A [productions] is a list of possible [production]s; a
-        [production] is a list of [item]s.  A string matches a
-        [production] if it can be broken up into components that match
-        the relevant element of the [production]. *)
-    Definition production := list item.
-    Definition productions := list production.
-
-    Definition productions_dec (CharType_eq_dec : forall x y : CharType, {x = y} + {x <> y})
-               (x y : productions) : {x = y} + {x <> y}.
-    Proof.
-      repeat (apply list_eq_dec; intros);
-      decide equality.
-      apply string_dec.
-    Defined.
-
-    (** A [grammar] consists of [productions] to match a string
-        against, and a function mapping names to [productions]. *)
-    (** TODO(jgross): also include list of valid starting non-terminals, for convenience and notation *)
-    (** TODO(jgross): look up notations for specifying these nicely *)
-    Record grammar :=
-      {
-        Start_symbol :> string;
-        Lookup :> string -> productions;
-        Start_production :> productions := Lookup Start_symbol;
-        Valid_nonterminal_symbols : list string;
-        Valid_nonterminals : list productions := map Lookup Valid_nonterminal_symbols
-      }.
-  End definitions.
-
+    Definition minimal_parse_of_item__of__parse_of_item
+               {str : String} {it : item CharType}
+               (p : parse_of_item String G str it)
+               (H : Forall_parse_of_item P p)
+    : minimal_parse_of_item initial_productions_data str it
+      := match @minimal_parse_of_item__of__parse_of_item'
+                 str initial_productions_data it
+                 _ (@minimal_parse_of__of__parse_of' _) p
+                 (Lt.lt_n_Sn _)
+                 H with
+           | inl p' => projT1 p'
+           | inr other => let H' := fst (projT2 other) in
+                          match Bool.eq_true_false_abs _ (proj2 H') (proj1 H') : False with end
+         end.
+  End minimize.
 End cfg.
-
-Arguments parse_of _%type_scope _ _ _%string_like _.
-Arguments parse_of_item _%type_scope _ _ _%string_like _.
-Arguments parse_of_production _%type_scope _ _ _%string_like _.
-Arguments parse_of_grammar _%type_scope _ _%string_like _.
-Section sound.
